Spontane kk in een bakje

heapsort.dfy
@@ -34,6 +34,13 @@ predicate heap(a: array<int>, end: int)
   forall i :: 0 < i <= end ==> a[parent(i)] >= a[i]
 }
 
+predicate heapWithoutBubble(a: array<int>, end: int, skip: int)
+  reads a
+  requires 0 <= end < a.Length
+{
+  forall i :: (0 < i <= end && i != skip) ==> a[parent(i)] >= a[i]
+}
+
 // parent node id in the tree
 function method parent(i: int) : int
 { (i - 1) / 2 }
@@ -62,12 +69,61 @@ lemma {:verify true} HeapMax(a: array<int>, i: int)
   requires heap(a, i)
   ensures firstmax(a, i)
 
+
 // turn a into a heap by bubbling up
 method {:verify true} Heapify(a: array<int>)
   modifies a;
   requires a.Length > 0;
   ensures heap(a, a.Length - 1);
   ensures multiset(a[..]) == multiset(old(a[..]));
+  {
+    var index: int := 1;
+    while (true)
+      decreases a.Length - index;
+      invariant multiset(a[..]) == multiset(old(a[..]));
+      invariant  1 <= index <= a.Length;
+      // invariant heap(a, index - 1);
+      // invariant firstmax(a, index);
+      // invariant a[parent(parent(index))] > a[parent(index)];
+      invariant forall i | 1 < i < index && parent(i) != 0 && parent(parent(i)) != 0 :: a[parent(parent(i))] > a[parent(i)];
+    {
+      if (index >= a.Length) {
+        break;
+      }
+
+      assert heap(a, 0) ==> firstmax(a, 0);
+      assert heap(a, 1) ==> firstmax(a, 1);
+
+      var updateIndex := index;
+      while (updateIndex > 0)
+        decreases updateIndex;
+        invariant multiset(a[..]) == multiset(old(a[..]));
+
+        invariant heap(a, updateIndex) ==> firstmax(a, updateIndex - 1);
+        // invariant 1 < updateIndex == index ==>  a[updateIndex] > a[parent(updateIndex)] || (heapWithoutBubble(a, updateIndex, updateIndex));
+        // invariant 1 < updateIndex < index ==> a[updateIndex] > a[parent(updateIndex)] || (heapWithoutBubble(a, updateIndex, updateIndex));
+        // invariant heapWithoutBubble(a, updateIndex, updateIndex)
+        // invariant heap(a, updateIndex - 1);
+      {
+        var parentIndex: int := parent(updateIndex);       
+
+        assert parentIndex < updateIndex;
+        assert updateIndex != 0;
+        assert heap(a, updateIndex) ==> a[lchild(0)] <= a[0];
+        // assert  updateIndex == index ==> ((a[updateIndex] >= a[parent(updateIndex)]) || (heap(a, updateIndex)));
+
+        if (a[updateIndex] > a[parentIndex]) {
+          a[updateIndex], a[parentIndex] := a[parentIndex], a[updateIndex];
+          assert a[updateIndex] <= a[parentIndex];
+          updateIndex := parentIndex;
+        } else {
+          break;
+        }
+      }
+      index := index + 1;
+    }
+
+  }
 
 
 // turn a into a sorted array by putting the head of a to the end
